kk

examples/n_german/n_mutualEx_base.thy
@@ -241,9 +241,9 @@ definition rulesOfPP1 :: "nat \<Rightarrow> rule set" where [simp]:
 
 definition rulesOfPP2 :: "nat \<Rightarrow> rule set" where [simp]:
   "rulesOfPP2 N \<equiv> {r.
-    (\<exists>i. i \<le> N \<and> r = n_Try i) \<or>
-    (\<exists>i. i \<le> N \<and> r = n_Crit i) \<or>
-    (\<exists>i. i \<le> N \<and> r = n_Exit i) \<or>
+    (\<exists>i. i \<le> N \<and> r = strengthenR2 [] [] (n_Try i)) \<or>
+    (\<exists>i. i \<le> N \<and> r = strengthenR2 [] [] (n_Crit i)) \<or>
+    (\<exists>i. i \<le> N \<and> r =  strengthenR2 [] [] (n_Exit i)) \<or>
     (\<exists>i. i \<le> N \<and> r = n_Idle_PP2 N i) 
    }"
 
@@ -551,34 +551,34 @@ proof (simp only: symProtRules'_def, (rule allI)+, rule impI)
   show "\<exists>r'. alphaEqRule r' (applySym2Rule p r) \<and> r' \<in> rulesOfPP2 N"
   proof -
     have b1: 
-     "(\<exists>i. i \<le> N \<and> r = n_Try i) \<or>
-      (\<exists>i. i \<le> N \<and> r = n_Crit i) \<or>
-      (\<exists>i. i \<le> N \<and> r = n_Exit i) \<or>
+     "(\<exists>i. i \<le> N \<and> r = strengthenR2 [] [] (n_Try i)) \<or>
+      (\<exists>i. i \<le> N \<and> r = strengthenR2 [] [] (n_Crit i)) \<or>
+      (\<exists>i. i \<le> N \<and> r = strengthenR2 [] [] (n_Exit i)) \<or>
       (\<exists>i. i \<le> N \<and> r = n_Idle_PP2 N i)"
       using local.a1 by auto
     moreover
-    {assume b1:"\<exists> i. i\<le>N\<and>r=n_Try  i"
-      from b1 obtain i where b1:"i\<le>N\<and>r=n_Try  i"
+    {assume b1:"\<exists> i. i\<le>N\<and>r=strengthenR2 [] [] (n_Try i)"
+      from b1 obtain i where b1:"i\<le>N\<and>r=strengthenR2 [] [] (n_Try i)"
         by blast
       from a1 have b2:"p i \<le> N"
         by (metis (mono_tags, lifting) b1 mem_Collect_eq permutes_def permutes_in_image)
-      from b1 have b3:"applySym2Rule p r= n_Try  ( p i)" 
+      from b1 have b3:"applySym2Rule p r= strengthenR1 [] [] (n_Try ( p i))" 
         by auto
-      have "applySym2Rule p r \<in> rules N "
+      have "applySym2Rule p r \<in> rulesOfPP1 N" 
         by (simp add: b2 b3)
       then have "\<exists>r'. alphaEqRule r' (applySym2Rule p r) \<and> r' \<in> rulesOfPP2 N"
         apply(rule_tac x="applySym2Rule p r" in exI)
         by (simp add: b3)
     }   
     moreover
-    {assume b1:"\<exists> i. i\<le>N\<and>r=n_Crit  i"
-      from b1 obtain i where b1:"i\<le>N\<and>r=n_Crit  i"
+    {assume b1:"\<exists> i. i\<le>N\<and>r=strengthenR2 [] [] (n_Crit  i)"
+      from b1 obtain i where b1:"i\<le>N\<and>r=strengthenR2 [] [] (n_Crit  i)"
         by blast
       from a1 have b2:"p i \<le> N"
         by (metis (mono_tags, lifting) b1 mem_Collect_eq permutes_def permutes_in_image)
-      from b1 have b3:"applySym2Rule p r= n_Crit  ( p i)" 
+      from b1 have b3:"applySym2Rule p r= strengthenR1 [] [] (n_Crit ( p i))" 
         by auto
-      have "applySym2Rule p r \<in> rules N "
+      have "applySym2Rule p r \<in> rulesOfPP2 N" 
         by (simp add: b2 b3)
       then have "\<exists>r'. alphaEqRule r' (applySym2Rule p r) \<and> r' \<in> rulesOfPP2 N"
         apply(rule_tac x="applySym2Rule p r" in exI)
@@ -692,19 +692,20 @@ proof (simp only: symProtRules'_def, (rule allI)+, rule impI)
        
     }
     moreover
-    {assume b1:"\<exists> i. i\<le>N\<and>r=n_Exit  i"
-      from b1 obtain i where b1:"i\<le>N\<and>r=n_Exit  i"
+    { 
+     assume b1:"\<exists> i. i\<le>N\<and>r=strengthenR2 [] [] (n_Exit  i)"
+      from b1 obtain i where b1:"i\<le>N\<and>r=strengthenR2 [] [] (n_Exit  i)"
         by blast
       from a1 have b2:"p i \<le> N"
         by (metis (mono_tags, lifting) b1 mem_Collect_eq permutes_def permutes_in_image)
-      from b1 have b3:"applySym2Rule p r= n_Exit  ( p i)" 
+      from b1 have b3:"applySym2Rule p r= strengthenR1 [] [] (n_Exit ( p i))" 
         by auto
-      have "applySym2Rule p r \<in> rules N "
+      have "applySym2Rule p r \<in> rulesOfPP2 N" 
         by (simp add: b2 b3)
-
-     then have "\<exists>r'. alphaEqRule r' (applySym2Rule p r) \<and> r' \<in> rulesOfPP2 N"
+      then have "\<exists>r'. alphaEqRule r' (applySym2Rule p r) \<and> r' \<in> rulesOfPP2 N"
         apply(rule_tac x="applySym2Rule p r" in exI)
         by (simp add: b3)
+       
     }
     ultimately show "\<exists>r'. alphaEqRule r' (applySym2Rule p r) \<and> r' \<in> rulesOfPP2 N"
       by blast
@@ -791,14 +792,21 @@ subsection\<open>Definitions of initial states
 
 lemma absMutualSimmutualPP2:
   assumes a1:"s \<in> reachableSetUpTo (andList (allInitSpecs N)) (rulesOfPP2 N) i" and a2:"N>1"
-  shows "s \<in> reachableSetUpTo (andList (allInitSpecs NC)) (rulesAbs NC) i \<and> (\<forall>f. f \<in> invariants NC \<longrightarrow> formEval f s)"
+  shows "s \<in> reachableSetUpTo (andList (allInitSpecs NC)) (rulesAbs NC) i \<and>
+ (\<forall>f. f \<in> invariants N \<longrightarrow> formEval f s)"
   sorry
 text \<open>
 1.mutualPP1 can simulate mutualPP2\<close> 
 
+lemma mutualPP2SatAllForm:
+  assumes a1:"s \<in> reachableSetUpTo (andList (allInitSpecs N)) (rulesOfPP2 N) i" and a2:"N>1"
+  shows " (\<forall>f. f \<in> invariants N \<longrightarrow> formEval f s)"
+  using a2 absMutualSimmutualPP2 local.a1 by blast
+
 lemma mutualPP2SimMutualPP1:
-  assumes a1:"s \<in> reachableSetUpTo (andList (allInitSpecs N)) (rulesOfPP1 N) i"
-  shows "s \<in> reachableSetUpTo (andList (allInitSpecs N)) (rulesOfPP2 N) i \<and> (\<forall>f. f \<in> invariants NC \<longrightarrow> formEval f s)"
+  assumes a1:"s \<in> reachableSetUpTo (andList (allInitSpecs N)) (rulesOfPP1 N) i" and a2:" N>1"
+  shows "s \<in> reachableSetUpTo (andList (allInitSpecs N)) (rulesOfPP2 N) i \<and>
+   (\<forall>f. f \<in> invariants N \<longrightarrow> formEval f s)"
   proof -
   let ?rs1="(rulesOfPP1 N)"
   let ?rs2="(rulesOfPP2 N)"
@@ -826,60 +834,64 @@ lemma mutualPP2SimMutualPP1:
         apply(rule_tac x="(n_Try i)" in exI)
         apply(rule_tac x="[]" in exI)
         apply(rule_tac x="[]" in exI)
-        apply simp
+       by simp
         
     }   
     moreover
-    {assume b1:"\<exists> i. i\<le>N\<and>r=n_Crit  i" 
-      from b1 obtain i where c1:"i\<le>N\<and>r=n_Crit  i"
+    {assume b1:"\<exists> i. i\<le>N\<and>r1=strengthenR1 [] [] (n_Crit  i)" 
+      from b1 obtain i where c1:"i\<le>N\<and>r1=strengthenR1 [] [] (n_Crit  i)"
         by blast
-      have "?post r"
+      have "?post r1"
         apply (cut_tac c1)
+        apply(rule_tac x="(n_Crit  i)" in exI)
         apply(rule_tac x="[]" in exI)
         apply(rule_tac x="[]" in exI)
         by simp
     }
     moreover
-    {assume b1:"\<exists> i. i\<le>N\<and>r=n_Idle i  "
-      from b1 obtain i where c1:"i\<le>N\<and>r=n_Idle i "
+    {assume b1:"\<exists> i. i\<le>N\<and>r1=n_Idle_PP1 N i  "
+      from b1 obtain i where c1:"i\<le>N\<and>r1=n_Idle_PP1 N i "
         by blast
        
-      have "?post r"
+      have "?post r1"
         apply (cut_tac c1)
+        apply(rule_tac x="(n_Idle  i)" in exI)
         apply(rule_tac x="(n_Idle_Ls1 N i)" in exI)
         apply(rule_tac x="[]" in exI)
-        apply(simp only:n_Idle_PP1_def)
+        apply(simp only:n_Idle_PP2_def)
         apply( auto simp del:n_Idle_def )
         using iINDown apply blast
         using iINDown apply blast  
         done
     }
     moreover
-    {assume b1:"\<exists> i. i\<le>N\<and>r=n_Exit  i"
-      from b1 obtain i where c1:"i\<le>N\<and>r=n_Exit  i"
+    {assume b1:"\<exists> i. i\<le>N\<and>r1=strengthenR1 [] [] (n_Exit   i)"
+      from b1 obtain i where c1:"i\<le>N\<and>r1=strengthenR1 [] [] (n_Exit   i)"
         by blast
-       have "?post r"
-        apply (cut_tac c1)
+       have "?post r1"
+       apply (cut_tac c1)
+        apply(rule_tac x="(n_Exit  i)" in exI)
         apply(rule_tac x="[]" in exI)
         apply(rule_tac x="[]" in exI)
-        by simp
+       by simp
     }
-    ultimately show "?post r"
+    ultimately show "?post r1"
       by blast
   qed
-  have b2:"\<forall>i s f. s \<in>reachableSetUpTo ?I ?rs' i \<longrightarrow> f \<in>?S \<longrightarrow>formEval f s"
-    using a2 mutualPP1SatAllForm by blast  
+  have b2:"\<forall>i s f. s \<in>reachableSetUpTo ?I ?rs2 i \<longrightarrow> f \<in>?S \<longrightarrow>formEval f s"
+    using a2 mutualPP2SatAllForm by blast  
  
     
 
-  show  "s \<in> reachableSetUpTo (andList (allInitSpecs N)) (rulesOfPP1 N) i \<and> (\<forall>f. f \<in> invariants N \<longrightarrow> formEval f s)"
-      using b1 b2 local.a1 strengthenProtSimProt1 by blast 
+  show  "s \<in> reachableSetUpTo (andList (allInitSpecs N)) (rulesOfPP2 N) i \<and> (\<forall>f. f \<in> invariants N \<longrightarrow> formEval f s)"
+      using b1 b2 local.a1 strengthenProtSimProt12 by blast 
   qed
 
 lemma mutualPP1SatAllForm:
   assumes a1:"s \<in> reachableSetUpTo (andList (allInitSpecs N)) (rulesOfPP1 N) i" and a2:"N>1"
   shows " (\<forall>f. f \<in> invariants N \<longrightarrow> formEval f s)"
-  sorry
+  using a2 local.a1 mutualPP2SimMutualPP1 by blast
+  
 lemma mutualPP1SimMutual:
   assumes a1:"s \<in> reachableSetUpTo (andList (allInitSpecs N)) (rules N) i" and a2:"N>1"
   shows "s \<in> reachableSetUpTo (andList (allInitSpecs N)) (rulesOfPP1 N) i \<and> (\<forall>f. f \<in> invariants N \<longrightarrow> formEval f s)"
